Structures/Trich2.v
@@ -1,0 +1,172 @@
+Require Export RCCBase.
+
+Set Implicit Arguments. 
+
+Class TrichDec : Type :=
+{
+    carrier : Type;
+    trich_lt : carrier -> carrier -> Prop;
+    (* trich_lt_antisym :
+      forall x y : carrier, trich_lt x y -> ~ trich_lt y x;
+     *)trich_lt_trans :
+      forall x y z : carrier, trich_lt x y -> trich_lt y z -> trich_lt x z;
+    trichb : carrier -> carrier -> comparison;
+    trichb_spec :
+      forall x y : carrier, CompareSpec (x = y) (trich_lt x y) (trich_lt y x) (trichb x y);
+    CompOpp_trichb :
+      forall x y : carrier,
+        CompOpp (trichb x y) = trichb y x;
+}.
+
+Hint Resolve trich_lt_trans : core.
+
+Definition TrichDec_ltb {A : TrichDec} (x y : @carrier A) : bool :=
+match trichb x y with
+    | Lt => true
+    | _ => false
+end.
+
+Definition TrichDec_le {A : TrichDec} (x y : @carrier A) : Prop :=
+  trich_lt x y \/ x = y.
+
+Definition TrichDec_leb {A : TrichDec} (x y : @carrier A) : bool :=
+match trichb x y with
+    | Lt | Eq => true
+    | Gt      => false
+end.
+
+Infix "<?>" := trichb (at level 70).
+Infix "<?" := TrichDec_ltb (at level 70).
+Infix "x ?> y" := (TrichDec_ltb y x) (at level 70).
+Infix "<=?" := TrichDec_leb (at level 70).
+Infix "x >=? y" := (TrichDec_leb y x) (at level 70).
+
+Infix "<" := trich_lt (at level 70).
+Infix "x > y" := (trich_lt y x) (at level 70).
+Infix "<=" := TrichDec_le (at level 70).
+Infix "x >= y" := (TrichDec_le y x) (at level 70).
+
+Require Import Equality.
+
+Lemma trich_lt_irrefl' :
+  forall (A : TrichDec) (x : carrier),
+    ~ trich_lt x x.
+Proof.
+  intros A x H. Check trichb_spec.
+  destruct (trichb_spec x x).
+  pose (Hxx := trichb_spec x x). inv Hxx.
+    pose (H0' := H0). apply (f_equal CompOpp) in H0'.
+      cbn in H0'. rewrite CompOpp_trichb in H0'. congruence.
+  destruct (trichb_spec x x) eqn: Hxx.
+Qed.
+
+
+Lemma trich_lt_antisym :
+  forall (A : TrichDec) (x y : carrier),
+    trich_lt x y -> ~ trich_lt y x.
+Proof.
+  intros A x y Hxy Hyx.
+  remember (trichb_spec x y) as Hxy'.
+  remember (trichb_spec y x) as Hyx'.
+  dependent destruction Hxy'.
+  dependent destruction Hyx'. Focus 4.
+  apply (f_equal CompOpp) in x1;
+  rewrite CompOpp_trichb in x1; cbn in *.
+    all: try congruence.
+Admitted.
+  
+  dependent destruction (trichb_spec x y). eqn: Hxy'.
+           (trichb_Spec y x) eqn: Hyx'.
+    
+Lemma trich_lt_irrefl :
+  forall (A : TrichDec) (x : carrier),
+    ~ trich_lt x x.
+Proof.
+  intros A x H. eapply trich_lt_antisym; eassumption.
+Qed.
+
+Hint Extern 0 =>
+match goal with
+    | H : _ < _ |- _ => apply trich_lt_irrefl in H; contradiction
+end
+  : core.
+
+Lemma trich_lt_antisym' :
+  forall (A : TrichDec) (x y : carrier),
+    trich_lt x y -> ~ trich_lt y x.
+Proof.
+  intros A x y.
+  intros Hxy Hyx.
+  eapply trich_lt_irrefl, trich_lt_trans; eassumption.
+Qed.
+
+Lemma trich_lt_comparison :
+  forall (A : TrichDec) (x y z : carrier),
+    trich_lt x z -> trich_lt x y \/ trich_lt y z.
+Proof.
+  intros. destruct (trichb_spec x y).
+    auto.
+    subst. auto.
+    right. eapply trich_lt_trans; eassumption.
+Qed.
+
+Lemma trich_lt_trans' :
+  forall (A : TrichDec) (x y z : carrier),
+    trich_lt x y -> trich_lt y z -> trich_lt x z.
+Proof.
+  intros A x y z Hxy Hyz.
+  destruct (trichb_spec x z).
+    assumption.
+    subst. contradict Hyz. apply trich_lt_antisym. assumption.
+    destruct (trich_lt_comparison _ _ z y Hxy).
+      assumption.
+      contradict H0. apply trich_lt_antisym. assumption.
+Qed.
+
+Lemma trich_lt_connected :
+  forall (A : TrichDec) (x y : carrier),
+    ~ trich_lt x y -> ~ trich_lt y x -> x = y.
+Proof.
+  intros. destruct (trichb_spec x y).
+    contradiction.
+    assumption.
+    contradiction.
+Qed.
+
+Hint Resolve trich_lt_irrefl trich_lt_comparison trich_lt_trans trich_lt_connected : core.
+
+Lemma trichb_spec1 :
+  forall (A : TrichDec) (x y : carrier),
+    trichb x y = Lt <-> trich_lt x y.
+Proof.
+  intros. destruct (trichb_spec x y);
+  subst; firstorder; try congruence.
+    contradict H0. apply trich_lt_antisym. assumption.
+Qed.
+
+Lemma trichb_spec2 :
+  forall (A : TrichDec) (x y : carrier),
+    trichb x y = Eq <-> x = y.
+Proof.
+  intros. destruct (trichb_spec x y);
+  firstorder; subst; auto; congruence.
+Qed.
+
+Lemma trichb_spec3 :
+  forall (A : TrichDec) (x y : carrier),
+    trichb x y = Gt <-> trich_lt y x.
+Proof.
+  intros. destruct (trichb_spec x y);
+  firstorder; try congruence.
+    contradict H0. apply trich_lt_antisym. assumption.
+    contradict H0. subst. apply trich_lt_irrefl.
+Qed.
+
+Lemma trich_lt_trich :
+  forall (A : TrichDec) (x y : carrier),
+    trich_lt x y \/ x = y \/ trich_lt y x.
+Proof.
+  intros. destruct (trichb_spec x y); auto.
+Qed.
+
+Hint Resolve trichb_spec1 trichb_spec2 trichb_spec3 trich_lt_trich : core.
